Prove bounded fresh-name search interface

venom/defs/irSupplyScript.sml
@@ -5,6 +5,8 @@
 Theory irSupply
 Ancestors
   venomCompilerWf
+  ASCIInumbers
+  pred_set
 Libs
   listTheory
 
@@ -157,6 +159,106 @@ Proof
        data_item_ir_labels_def, MEM_FLAT, MEM_MAP, PULL_EXISTS] >>
   disj2_tac >> qexists `section` >> simp[] >>
   disj2_tac >> qexists `DataLabel l` >> simp[data_item_ir_labels_def]
+QED
+
+Definition fresh_name_candidate_def:
+  fresh_name_candidate prefix (n:num) = STRCAT prefix (toString n)
+End
+
+Definition seek_fresh_name_def:
+  seek_fresh_name prefix used n 0 = (fresh_name_candidate prefix n,n) /\
+  seek_fresh_name prefix used n (SUC fuel) =
+    if MEM (fresh_name_candidate prefix n) used then
+      seek_fresh_name prefix used (SUC n) fuel
+    else (fresh_name_candidate prefix n,n)
+End
+
+Theorem seek_fresh_name_shape:
+  seek_fresh_name prefix used n fuel = (name,k) ==>
+  name = fresh_name_candidate prefix k /\
+  n <= k /\ k <= n + fuel
+Proof
+  qid_spec_tac `n` >> Induct_on `fuel`
+  >- simp[seek_fresh_name_def]
+  >> gen_tac >>
+  Cases_on `MEM (fresh_name_candidate prefix n) used`
+  >- (simp[seek_fresh_name_def] >> strip_tac >>
+      first_x_assum drule >> strip_tac >> simp[] >> decide_tac)
+  >> simp[seek_fresh_name_def] >> strip_tac >> gvs[]
+QED
+
+Theorem fresh_name_candidates_distinct:
+  !prefix n count.
+  ALL_DISTINCT
+    (GENLIST (\i. fresh_name_candidate prefix (n + i)) count)
+Proof
+  simp[ALL_DISTINCT_GENLIST, fresh_name_candidate_def] >>
+  decide_tac
+QED
+
+Theorem distinct_members_length_le:
+  ALL_DISTINCT xs /\ EVERY (\x. MEM x ys) xs ==>
+  LENGTH xs <= LENGTH ys
+Proof
+  strip_tac >>
+  `set xs SUBSET set ys` by gvs[SUBSET_DEF, EVERY_MEM] >>
+  `CARD (set xs) <= CARD (set ys)` by
+    (irule CARD_SUBSET >> simp[]) >>
+  drule ALL_DISTINCT_CARD_LIST_TO_SET >> strip_tac >> gvs[] >>
+  `CARD (set ys) <= LENGTH ys` by simp[CARD_LIST_TO_SET] >>
+  decide_tac
+QED
+
+Theorem seek_fresh_name_checked:
+  MEM (FST (seek_fresh_name prefix used n fuel)) used ==>
+  !i. i <= fuel ==> MEM (fresh_name_candidate prefix (n + i)) used
+Proof
+  qid_spec_tac `n` >> Induct_on `fuel`
+  >- simp[seek_fresh_name_def]
+  >> gen_tac >>
+  Cases_on `MEM (fresh_name_candidate prefix n) used`
+  >- (simp[seek_fresh_name_def] >> strip_tac >>
+      Cases_on `i` >- simp[] >>
+      rename1 `SUC j <= SUC fuel` >>
+      first_x_assum drule >> strip_tac >> strip_tac >>
+      qpat_assum `!i. i <= fuel ==> _` (qspec_then `j` mp_tac) >>
+      impl_tac >- decide_tac >> strip_tac >>
+      `SUC n + j = SUC j + n` by decide_tac >> gvs[])
+  >> simp[seek_fresh_name_def]
+QED
+
+Theorem seek_fresh_name_fresh:
+  ~MEM (FST (seek_fresh_name prefix used n (LENGTH used))) used
+Proof
+  strip_tac >>
+  `EVERY (\x. MEM x used)
+     (GENLIST (\i. fresh_name_candidate prefix (n + i))
+              (SUC (LENGTH used)))` by
+    (simp[EVERY_GENLIST] >> rpt strip_tac >>
+     drule seek_fresh_name_checked >>
+     disch_then (qspec_then `i` mp_tac) >>
+     impl_tac >- decide_tac >> strip_tac >>
+     `n + i = i + n` by decide_tac >> gvs[]) >>
+  `ALL_DISTINCT
+     (GENLIST (\i. fresh_name_candidate prefix (n + i))
+              (SUC (LENGTH used)))` by
+    simp[fresh_name_candidates_distinct] >>
+  drule_all distinct_members_length_le >> simp[]
+QED
+
+Theorem seek_fresh_name_interface:
+  seek_fresh_name prefix used n (LENGTH used) = (name,k) ==>
+  name = STRCAT prefix (toString k) /\
+  n <= k /\ k <= n + LENGTH used /\
+  ~MEM name used
+Proof
+  strip_tac >>
+  `name = fresh_name_candidate prefix k /\
+   n <= k /\ k <= n + LENGTH used` by
+    (drule seek_fresh_name_shape >> simp[]) >>
+  `~MEM (FST (seek_fresh_name prefix used n (LENGTH used))) used` by
+    simp[seek_fresh_name_fresh] >>
+  gvs[fresh_name_candidate_def]
 QED
 
 val _ = export_theory ();
